src/StepDet.v
@@ -11,7 +11,7 @@ Fixpoint getTMsgsTInfo (tmsgs: list TMsg) :=
     end
   end.
 
-Inductive step_det (sys: System OrdOState): TState -> TLabel -> TState -> Prop :=
+Inductive step_det (sys: System): TState -> TLabel -> TState -> Prop :=
 | SdSlt: forall st, step_det sys st emptyRLabel st
 | SdExt: forall ts oss oims emsg,
     isExternal sys (mid_from (msg_id emsg)) = true ->
@@ -27,15 +27,13 @@ Inductive step_det (sys: System OrdOState): TState -> TLabel -> TState -> Prop :
                 tst_tid := ts
              |}
 | SdInt: forall ts nts (Hts: nts > ts) tinfo
-                oss oims obj oidx os pos msgs rule outs,
-    In obj sys ->
-    oidx = obj_idx obj ->
+                oss oims oidx os pos msgs rule outs,
+    In oidx (indicesOf sys) ->
     (oss)@[oidx] = Some os ->
-
     Forall (FirstMP oims) msgs ->
     ValidMsgsIn oidx msgs ->
     map (fun tmsg => msg_id (tmsg_msg tmsg)) msgs = rule_mids rule ->
-    In rule (obj_rules obj) ->
+    In rule (sys_rules sys) ->
     rule_precond rule os (map tmsg_msg msgs) ->
     rule_postcond rule os (map tmsg_msg msgs) pos outs ->
     ValidMsgOuts oidx outs ->
@@ -61,5 +59,5 @@ Inductive step_det (sys: System OrdOState): TState -> TLabel -> TState -> Prop :
                            end
              |}.
 
-Definition steps_det: Steps (System OrdOState) TState TLabel := steps step_det.
+Definition steps_det: Steps System TState TLabel := steps step_det.
 
