src/SynthesisFacts.v
@@ -3,62 +3,37 @@ Require Import Common FMap ListSupport Syntax Wf Semantics SemFacts StepDet Synt
 Require Import Serial SerialFacts Simulation TrsInv TrsSim.
 
 Lemma addRules_init:
-  forall rules objs,
-    getObjectStatesInit (addRules rules objs) =
-    getObjectStatesInit objs.
-Proof.
-  induction objs; simpl; intros; [reflexivity|].
-  rewrite IHobjs.
-  reflexivity.
-Qed.
-
-Lemma addRulesSys_init:
   forall rules sys,
-    getStateInit (StateT:= TState) (addRulesSys rules sys) =
-    getStateInit (StateT:= TState) sys.
+    initsOf (StateT:= TState) (addRules rules sys) =
+    initsOf (StateT:= TState) sys.
 Proof.
-  unfold addRulesSys; simpl; intros.
-  unfold getTStateInit; simpl.
-  rewrite addRules_init.
   reflexivity.
 Qed.
 
 Lemma addRules_indices:
-  forall rules objs,
-    map (fun o => obj_idx o) (addRules rules objs) =
-    map (fun o => obj_idx o) objs.
+  forall rules sys,
+    indicesOf (addRules rules sys) = indicesOf sys.
 Proof.
-  induction objs; simpl; intros; [reflexivity|].
-  rewrite IHobjs.
   reflexivity.
 Qed.
 
-Lemma addRulesSys_indices:
+Corollary addRules_isExternal:
   forall rules sys,
-    indicesOf (addRulesSys rules sys) = indicesOf sys.
-Proof.
-  unfold addRulesSys; simpl; intros.
-  unfold indicesOf; simpl.
-  apply addRules_indices.
-Qed.
-
-Corollary addRulesSys_isExternal:
-  forall rules sys,
-    isExternal (addRulesSys rules sys) =
+    isExternal (addRules rules sys) =
     isExternal sys.
 Proof.
   unfold isExternal; intros.
-  rewrite addRulesSys_indices.
+  rewrite addRules_indices.
   reflexivity.
 Qed.
   
-Corollary addRulesSys_isInternal:
+Corollary addRules_isInternal:
   forall rules sys,
-    isInternal (addRulesSys rules sys) =
+    isInternal (addRules rules sys) =
     isInternal sys.
 Proof.
   unfold isInternal; intros.
-  rewrite addRulesSys_indices.
+  rewrite addRules_indices.
   reflexivity.
 Qed.
 
@@ -66,9 +41,7 @@ Lemma buildRawSys_indicesOf:
   forall sys, indicesOf sys = indicesOf (buildRawSys sys).
 Proof.
   intros; unfold indicesOf, buildRawSys; simpl.
-  induction sys; [reflexivity|].
-  unfold id in *.
-  simpl; rewrite IHsys; reflexivity.
+  reflexivity.
 Qed.
 
 Corollary buildRawSys_isExternal:
@@ -91,94 +64,20 @@ Proof.
   reflexivity.
 Qed.
 
-Lemma addRules_rule_in:
-  forall rule rules obs iobj,
-    In rule (obj_rules iobj) ->
-    In iobj (addRules rules obs) ->
-    exists obj : Object OrdOState,
-      obj_idx obj = obj_idx iobj /\
-      In rule (obj_rules obj) /\
-      In obj (obs ++ addRules rules (buildRawObjs obs)).
-Proof.
-  induction obs; simpl; intros; [intuition idtac|].
-  destruct H0; subst.
-  - clear IHobs.
-    unfold addRulesO in H; simpl in H.
-    apply in_app_or in H; destruct H.
-    + exists (addRulesO rules
-                        {| obj_idx := obj_idx a;
-                           obj_state_init := obj_state_init a;
-                           obj_rules := nil |}); simpl; repeat split.
-      * rewrite app_nil_r; assumption.
-      * right; apply in_or_app; right.
-        left; reflexivity.
-    + exists a; repeat split; auto.
-  - specialize (IHobs _ H H0).
-    destruct IHobs as [obj [? [? ?]]].
-    exists obj; repeat split; auto.
-    right.
-    apply in_or_app.
-    apply in_app_or in H3; destruct H3.
-    + left; assumption.
-    + right; right; auto.
-Qed.
-
-Lemma addRulesO_app:
-  forall obj rules1 rules2,
-    addRulesO (rules1 ++ rules2) obj = addRulesO rules1 (addRulesO rules2 obj).
-Proof.
-  unfold addRulesO; intros; simpl; f_equal.
-  rewrite filter_app.
-  apply eq_sym, app_assoc.
-Qed.
-  
 Lemma addRules_app:
-  forall obs rules1 rules2,
-    addRules (rules1 ++ rules2) obs =
-    addRules rules1 (addRules rules2 obs).
-Proof.
-  induction obs; simpl; intros; [reflexivity|].
-  rewrite addRulesO_app, IHobs; reflexivity.
-Qed.
-
-Lemma addRulesSys_app:
   forall sys rules1 rules2,
-    addRulesSys (rules1 ++ rules2) sys =
-    addRulesSys rules1 (addRulesSys rules2 sys).
+    addRules (rules1 ++ rules2) sys =
+    addRules rules2 (addRules rules1 sys).
 Proof.
-  unfold addRulesSys; intros; simpl.
-  rewrite addRules_app; reflexivity.
+  unfold addRules; simpl; intros.
+  rewrite app_assoc; reflexivity.
 Qed.
 
-Lemma addRulesSys_rule_in:
-  forall sys rules rule iobj,
-    In rule (obj_rules iobj) ->
-    In iobj (addRulesSys rules sys) ->
-    exists obj : Object OrdOState,
-      obj_idx obj = obj_idx iobj /\
-      In rule (obj_rules obj) /\
-      In obj (sys ++ (addRulesSys rules (buildRawSys sys))).
-Proof.
-  intros; simpl in *.
-  apply addRules_rule_in; auto.
-Qed.
-
-Lemma addRulesSys_buildRawSys_sublist:
+Lemma addRulesSys_buildRawSys:
   forall rules sys,
-    SubList (rulesOf (addRulesSys rules (buildRawSys sys)))
-            rules.
+    rulesOf (addRules rules (buildRawSys sys)) = rules.
 Proof.
-  unfold rulesOf; intros; simpl.
-  induction sys; [simpl; apply SubList_nil|].
-
-  simpl.
-  apply SubList_app_3; [|assumption].
-  apply SubList_app_3; [|apply SubList_nil].
-  clear; induction rules; [apply SubList_nil|].
-  simpl; find_if_inside.
-  - apply SubList_cons; [left; reflexivity|].
-    apply SubList_cons_right; assumption.
-  - apply SubList_cons_right; assumption.
+  reflexivity.
 Qed.
 
 Lemma rollbacked_enqMP_toTMsgU:
@@ -219,23 +118,17 @@ Corollary trsSimulates_trsInvHolds_rules_added:
          (Hsim1: TrsSimulates simR ginv simP impl spec)
          (Hinv1: TrsInv impl ginv)
          (Hmt1: trsPreservingSys impl)
-         (Hsim2: TrsSimulates simR ginv simP (addRulesSys rules (buildRawSys impl)) spec)
-         (Hinv1: TrsInv (addRulesSys rules (buildRawSys impl)) ginv)
-         (Hmt2: trsPreservingSys (addRulesSys rules (buildRawSys impl)))
+         (Hsim2: TrsSimulates simR ginv simP (addRules rules (buildRawSys impl)) spec)
+         (Hinv1: TrsInv (addRules rules (buildRawSys impl)) ginv)
+         (Hmt2: trsPreservingSys (addRules rules (buildRawSys impl)))
          (Hmtdisj: TrsDisj (rulesOf impl) rules),
-    TrsSimulates simR ginv simP (addRulesSys rules impl) spec /\
-    TrsInv (addRulesSys rules impl) ginv.
+    TrsSimulates simR ginv simP (addRules rules impl) spec /\
+    TrsInv (addRules rules impl) ginv.
 Proof.
   intros.
   eapply trsSimulates_trsInvHolds_compositional
-    with (impl1:= impl) (impl2:= addRulesSys rules (buildRawSys impl)); eauto.
-  - rewrite addRulesSys_indices.
-    apply buildRawSys_indicesOf.
-  - unfold TrsDisjSys.
-    eapply TrsDisj_SubList_2; eauto.
-    apply addRulesSys_buildRawSys_sublist.
-  - admit. (* should be easily derivable from [Hmt1] and [Hmt2] *)
-  - apply addRulesSys_indices.
-  - apply addRulesSys_rule_in; auto.
-Admitted.
+    with (impl1:= impl) (impl2:= addRules rules (buildRawSys impl)); eauto.
+  unfold addRules, trsPreservingSys in *; simpl in *.
+  apply Forall_app; auto.
+Qed.
 
